added an addition function and the skeleton of monoid instance

modexp.lean
@@ -1,7 +1,9 @@
 
 import data.bitvec
 
-def word_size := 32
+def word_size : ℕ := 32
+
+def num_vals : ℕ := 2^word_size
 
 @[reducible]
 def word := bitvec word_size
@@ -9,20 +11,94 @@ def word := bitvec word_size
 open nat
 
 def up {n : ℕ} : fin n → fin (succ n)
- | ⟨i,P⟩ := ⟨i,by { transitivity n, { apply P }, { apply nat.lt_succ_self } }⟩
-
-#check @array.read
+ | ⟨i,P⟩ := ⟨i,show i < succ n, by { transitivity n, { apply P }, { apply nat.lt_succ_self } }⟩
 
 structure bignum :=
   (cap  : ℕ)
   (size : fin (succ cap))
   (data : array word cap)
   (all_zero : ∀ i, size ≤ up i → data.read i = 0)
-  (msb_not_zero : ∀ last, fin.succ last = size → data.read last ≠ 0)
+  (msw_not_zero : ∀ last, fin.succ last = size → data.read last ≠ 0)
 
 namespace bignum
 
 def to_nat (n : bignum) : ℕ :=
 n.data.iterate 0 (λ i w r, r + w.to_nat * 2 ^ (i.val * word_size))
+
+def zero : bignum :=
+{ cap := 0
+, size := 0
+, data := ⟨ λ i, i.elim0 ⟩
+, all_zero := assume i, i.elim0
+, msw_not_zero := assume i, i.elim0
+}
+
+def words (p : bignum) (n : ℕ) : word :=
+if h : n < p.cap
+   then p.data.read ⟨n,h⟩
+   else 0
+
+namespace add
+
+def add_carry (p q : bignum) : ℕ → word
+ | 0 := 0
+ | (succ i) :=
+   let c := (add_carry i).to_nat,
+       x := (p.words $ succ i).to_nat,
+       y := (q.words $ succ i).to_nat in
+   if num_vals ≤ c + x + y
+      then 1
+      else 0
+
+def add_val (p q : bignum) (i : ℕ) : word :=
+p.words i + p.words i + add_carry p q i
+
+def msw_aux {n} (ar : array word n)
+: ∀ i, i < succ n → fin (succ n)
+| 0 P := ⟨ _, P ⟩
+| (succ i) P :=
+if ar.read ⟨i,lt_of_succ_lt_succ P⟩ = 0
+then msw_aux i (by { transitivity succ i, apply lt_succ_self, apply P })
+else ⟨succ i,P⟩
+
+def msw {n} (ar : array word n) : fin (succ n) :=
+msw_aux ar n (lt_succ_self _)
+
+lemma msw_not_zero {n} (ar : array word n)
+: ∀ last, fin.succ last = msw ar → ar.read last ≠ 0 :=
+sorry
+
+lemma msw_all_zero {n} (ar : array word n)
+: ∀ i, msw ar ≤ up i → ar.read i = 0 :=
+sorry
+
+def data {n} (p q : bignum) : array word n :=
+⟨ λ i , add_val p q i.val ⟩
+
+end add
+
+def add (p q : bignum) : bignum :=
+{ cap := max p.size.val q.size.val + 1
+, data := add.data p q
+, size := add.msw (add.data p q)
+, msw_not_zero := add.msw_not_zero (add.data p q)
+, all_zero := add.msw_all_zero (add.data p q) }
+
+instance : has_add bignum :=
+⟨ add ⟩
+
+theorem to_nat_add (p q : bignum)
+: (p + q).to_nat = p.to_nat + q.to_nat :=
+sorry
+
+-- todo: look into setoid
+-- the same nat can be represented by two different bignums
+-- by just padding the number with zeros
+instance : add_monoid bignum :=
+{ zero := zero
+, add := add
+, add_zero := sorry
+, zero_add := sorry
+, add_assoc := sorry }
 
 end bignum
